
\begin{equation}
\begin{split}
    \frac{\partial\psi}{\partial\phi}\frac{\partial}{\partial\lambda}\left(\frac{f}{H}\right) - \frac{\partial\psi}{\partial\lambda}\frac{\partial}{\partial\phi}\left(\frac{f}{H}\right) 
    = \frac{\partial}{\partial\phi}\frac{1}{H}\frac{\partial}{\partial\lambda}\left(\int_{-H}^0zb\, \text{d}z\right) - \frac{\partial}{\partial\lambda}\frac{1}{H}\frac{\partial}{\partial\phi}\left(\int_{-H}^0zb\, \text{d}z\right)  \\
    + \frac{a}{\rho_0}\left[\frac{\partial}{\partial\lambda}\left(\frac{\tau_\phi^s}{H}\right)-\frac{\partial}{\partial\phi}\left(\frac{\tau_\lambda^s\cos\phi}{H}\right)\right].
\end{split}
\label{EQN:FullCrossDifferential}
\end{equation}
